responded to changes

week-02/week2_refactoring.v
@@ -313,7 +313,8 @@ Proof.
   - rewrite -> fold_unfold_refactor_aux_Minus.
     rewrite ->2 fold_unfold_evaluate_Plus.
     rewrite ->2 fold_unfold_evaluate_Minus.
-    rewrite -> IHae1, IHae2.
+    rewrite -> (IHae1 (Literal 0)).
+    rewrite -> (IHae2 (Literal 0)).
     rewrite ->2 fold_unfold_evaluate_Plus.
     case (evaluate ae1) as [n1 | s1] eqn:E_ae1.
     + case (evaluate ae2) as [n2 | s2] eqn:E_ae2.
@@ -336,373 +337,7 @@ Proof.
   reflexivity.
 Qed.
 
-Proposition equivalence_of_the_two_lemmas_for_refactor_ind :
-  forall ae : arithmetic_expression,
-    (forall s : string,
-        evaluate ae = Expressible_msg s ->
-        forall a : arithmetic_expression,
-          evaluate (refactor_aux ae a) = Expressible_msg s)
-    /\
-      (forall (n : nat)
-              (s : string),
-          evaluate ae = Expressible_nat n ->
-          forall a : arithmetic_expression,
-            evaluate a = Expressible_msg s ->
-            evaluate (refactor_aux ae a) = Expressible_msg s)
-    /\
-      (forall n1 n2 : nat,
-          evaluate ae = Expressible_nat n1 ->
-          forall a : arithmetic_expression,
-            evaluate a = Expressible_nat n2 ->
-            evaluate (refactor_aux ae a) = Expressible_nat (n1 + n2))
-    <->
-      forall a : arithmetic_expression,
-        evaluate (refactor_aux ae a) = evaluate (Plus ae a).
-Proof.
-  intro ae.
-  split.
-  - intros _.
-    induction ae as [ n | ae1 IHae1 ae2 IHae2 | ae1 IHae1 ae2 IHae2 ];
-      intro a.
-    + rewrite -> fold_unfold_refactor_aux_Literal.
-      reflexivity.
-    + rewrite -> fold_unfold_refactor_aux_Plus.
-      rewrite -> (IHae1 (refactor_aux ae2 a)).
-      rewrite -> fold_unfold_evaluate_Plus.
-      rewrite -> (IHae2 a).
-      case (evaluate ae1) as [n1 | s1] eqn:E_ae1.
-      * rewrite ->3 fold_unfold_evaluate_Plus.
-        rewrite -> E_ae1.
-        case (evaluate ae2) as [n2 | s2] eqn:E_ae2.
-        -- case (evaluate a) as [n | s] eqn:E_a.
-           ++ rewrite -> Nat.add_assoc.
-              reflexivity.
-           ++ reflexivity.
-        -- reflexivity.
-      * rewrite ->2 fold_unfold_evaluate_Plus.
-        rewrite -> E_ae1.
-        reflexivity.
-    + rewrite -> fold_unfold_refactor_aux_Minus.
-      rewrite ->2 fold_unfold_evaluate_Plus.
-      rewrite ->2 fold_unfold_evaluate_Minus.
-      rewrite -> IHae1, IHae2.
-      rewrite ->2 fold_unfold_evaluate_Plus.
-      case (evaluate ae1) as [n1 | s1] eqn:E_ae1.
-      * case (evaluate ae2) as [n2 | s2] eqn:E_ae2.
-        -- rewrite -> fold_unfold_evaluate_Literal.
-           rewrite ->2 Nat.add_0_r.
-           reflexivity.
-        -- rewrite -> fold_unfold_evaluate_Literal.
-           reflexivity.
-      * reflexivity.
-  - induction ae as [ n | ae1 IHae1 ae2 IHae2 | ae1 IHae1 ae2 IHae2 ].
-    intros H_refactor.
-    split.
-    + intro s.
-      intro H_absurd.
-      discriminate H_absurd.
-    + split.
-      * intros n0 s_msg a ae H_ae.
-        case (evaluate ae) as [n_ae | s_ae] eqn:E_ae.
-        -- discriminate H_ae.
-        -- rewrite -> (H_refactor ae).
-           rewrite -> fold_unfold_evaluate_Plus.
-           rewrite -> fold_unfold_evaluate_Literal.
-           rewrite -> E_ae.
-           rewrite -> H_ae.
-           reflexivity.
-      * intros n1 n2 H_literal ae H_ae.
-        case (evaluate ae) as [n_ae | s_ae] eqn:E_ae.
-        -- rewrite -> fold_unfold_refactor_aux_Literal.
-           rewrite -> fold_unfold_evaluate_Plus.
-           rewrite -> H_literal.
-           rewrite -> E_ae.
-           injection H_ae.
-           intro H_eq_n_ae_n2.
-           rewrite -> H_eq_n_ae_n2.
-           reflexivity.
-        -- discriminate H_ae.
-    + intro H_refactor.
-      split.
-      * intros s H_plus.
-        destruct IHae1 as [IH1_ae1 [IH2_ae1 IH3_ae1]].
-        destruct IHae2 as [IH1_ae2 [IH2_ae2 IH3_ae2]].
-        -- intro ae.
-           rewrite -> (refactoring_preserves_evaluation_aux ae2 ae).
-           reflexivity.
-        -- intro ae.
-           rewrite -> (refactoring_preserves_evaluation_aux ae1 ae).
-           reflexivity.
-        -- intro ae.
-           case (evaluate ae1) as [n1 | s1] eqn:E_ae1.
-           case (evaluate ae2) as [n2 | s2] eqn:E_ae2.
-           case (evaluate ae) as [n_ae | s_ae] eqn:E_ae.
-           ++ rewrite -> fold_unfold_evaluate_Plus in H_plus.
-              rewrite -> E_ae2 in H_plus.
-              rewrite -> E_ae1 in H_plus.
-              discriminate H_plus.
-           ++ rewrite -> fold_unfold_evaluate_Plus in H_plus.
-              rewrite -> E_ae2 in H_plus.
-              rewrite -> E_ae1 in H_plus.
-              discriminate H_plus.
-           ++ rewrite -> fold_unfold_evaluate_Plus in H_plus.
-              rewrite -> E_ae2 in H_plus.
-              rewrite -> E_ae1 in H_plus.
-              rewrite -> (H_refactor ae).
-              rewrite -> 2 fold_unfold_evaluate_Plus.
-              rewrite -> E_ae2.
-              rewrite -> E_ae1.
-              rewrite -> H_plus.
-              reflexivity.
-           ++ rewrite -> fold_unfold_evaluate_Plus in H_plus.
-              rewrite -> E_ae1 in H_plus.
-              rewrite -> (H_refactor ae).
-              rewrite -> 2 fold_unfold_evaluate_Plus.
-              rewrite -> E_ae1.
-              rewrite -> H_plus.
-              reflexivity.
-    * split.
-      -- intros n s H_plus.
-         destruct IHae1 as [IH1_ae1 [IH2_ae1 IH3_ae1]].
-         destruct IHae2 as [IH1_ae2 [IH2_ae2 IH3_ae2]].
-         ++ intro ae.
-            rewrite -> (refactoring_preserves_evaluation_aux ae2 ae).
-            reflexivity.
-         ++ intro ae.
-            rewrite -> (refactoring_preserves_evaluation_aux ae1 ae).
-            reflexivity.
-         ++ intro ae.
-            case (evaluate ae1) as [n1 | s1] eqn:E_ae1.
-            case (evaluate ae2) as [n2 | s2] eqn:E_ae2.
-            case (evaluate ae) as [n_ae | s_ae] eqn:E_ae.
-            ** intro H_absurd.
-               discriminate H_absurd.
-            ** intro H_true.
-               rewrite -> (H_refactor ae).
-               rewrite -> 2 fold_unfold_evaluate_Plus.
-               rewrite -> E_ae2.
-               rewrite -> E_ae1.
-               rewrite -> E_ae.
-               exact (H_true).
-            ** intros _.
-               rewrite -> fold_unfold_evaluate_Plus in H_plus.
-               rewrite -> E_ae2 in H_plus.
-               rewrite -> E_ae1 in H_plus.
-               discriminate H_plus.
-            ** intros _.
-               rewrite -> fold_unfold_evaluate_Plus in H_plus.
-               rewrite -> E_ae1 in H_plus.
-               discriminate H_plus.
-      -- intros n1 n2 H_plus.
-         destruct IHae1 as [IH1_ae1 [IH2_ae1 IH3_ae1]].
-         destruct IHae2 as [IH1_ae2 [IH2_ae2 IH3_ae2]].
-         ++ intro ae.
-            rewrite -> (refactoring_preserves_evaluation_aux ae2 ae).
-            reflexivity.
-         ++ intro ae.
-            rewrite -> (refactoring_preserves_evaluation_aux ae1 ae).
-            reflexivity.
-         ++ intro ae.
-            case (evaluate ae1) as [n_ae1 | s_ae1] eqn:E_ae1.
-            case (evaluate ae2) as [n_ae2 | s_ae2] eqn:E_ae2.
-            case (evaluate ae) as [n_ae | s_ae] eqn:E_ae.
-            ** intro H_exp_n_ae_eq_exp_n2.
-               rewrite -> fold_unfold_evaluate_Plus in H_plus.
-               rewrite -> E_ae2 in H_plus.
-               rewrite -> E_ae1 in H_plus.
-               rewrite -> (H_refactor ae).
-               rewrite -> 2 fold_unfold_evaluate_Plus.
-               rewrite -> E_ae2.
-               rewrite -> E_ae1.
-               rewrite -> E_ae.
-               injection H_exp_n_ae_eq_exp_n2.
-               intro H_n_ae_eq_n2.
-               injection H_plus.
-               intro H_n_ae1_plus_n_ae2_eq_n1.
-               rewrite -> H_n_ae_eq_n2.
-               rewrite -> H_n_ae1_plus_n_ae2_eq_n1.
-               reflexivity.
-            ** intro H_absurd.
-               discriminate H_absurd.
-            ** intro H_ae.
-               rewrite -> fold_unfold_evaluate_Plus in H_plus.
-               rewrite -> E_ae2 in H_plus.
-               rewrite -> E_ae1 in H_plus.
-               discriminate H_plus.
-            ** intro H_ae.
-               rewrite -> fold_unfold_evaluate_Plus in H_plus.
-               rewrite -> E_ae1 in H_plus.
-               discriminate H_plus.
-    + intro H_refactor.
-      split.
-      * intros s H_minus.
-        destruct IHae1 as [IH1_ae1 [IH2_ae1 IH3_ae1]].
-        destruct IHae2 as [IH1_ae2 [IH2_ae2 IH3_ae2]].
-        -- intro ae.
-           rewrite -> (refactoring_preserves_evaluation_aux ae2 ae).
-           reflexivity.
-        -- intro ae.
-           rewrite -> (refactoring_preserves_evaluation_aux ae1 ae).
-           reflexivity.
-        -- intro ae.
-           case (evaluate ae1) as [n1 | s1] eqn:E_ae1.
-           case (evaluate ae2) as [n2 | s2] eqn:E_ae2.
-           case (evaluate ae) as [n_ae | s_ae] eqn:E_ae.
-           ++ rewrite -> (H_refactor ae).
-              rewrite -> fold_unfold_evaluate_Plus.
-              rewrite -> fold_unfold_evaluate_Minus.
-              rewrite -> E_ae.
-              rewrite -> E_ae2.
-              rewrite -> E_ae1.
-              case (n1 <? n2) eqn:E_lt.
-              ** rewrite -> fold_unfold_evaluate_Minus in H_minus.
-                 rewrite -> E_ae2 in H_minus.
-                 rewrite -> E_ae1 in H_minus.
-                 case (n1 <? n2) eqn:E_lt_minus.
-                 --- exact (H_minus).
-                 --- discriminate E_lt.
-              ** rewrite -> fold_unfold_evaluate_Minus in H_minus.
-                 rewrite -> E_ae2 in H_minus.
-                 rewrite -> E_ae1 in H_minus.
-                 case (n1 <? n2) eqn:E_lt_minus.
-                 --- discriminate E_lt.
-                 --- discriminate H_minus.
-           ++ rewrite -> (H_refactor ae).
-              rewrite -> fold_unfold_evaluate_Plus.
-              rewrite -> fold_unfold_evaluate_Minus.
-              rewrite -> E_ae.
-              rewrite -> E_ae2.
-              rewrite -> E_ae1.
-              case (n1 <? n2) eqn:E_lt.
-              ** rewrite -> fold_unfold_evaluate_Minus in H_minus.
-                 rewrite -> E_ae2 in H_minus.
-                 rewrite -> E_ae1 in H_minus.
-                 case (n1 <? n2) eqn:E_lt_minus.
-                 --- exact (H_minus).
-                 --- discriminate E_lt.
-              ** rewrite -> fold_unfold_evaluate_Minus in H_minus.
-                 rewrite -> E_ae2 in H_minus.
-                 rewrite -> E_ae1 in H_minus.
-                 case (n1 <? n2) eqn:E_lt_minus.
-                 --- discriminate E_lt.
-                 --- discriminate H_minus.
-           ++ rewrite -> fold_unfold_evaluate_Minus in H_minus.
-              rewrite -> E_ae2 in H_minus.
-              rewrite -> E_ae1 in H_minus.
-              rewrite -> (H_refactor ae).
-              rewrite -> fold_unfold_evaluate_Plus.
-              rewrite -> fold_unfold_evaluate_Minus.
-              rewrite -> E_ae2.
-              rewrite -> E_ae1.
-              exact (H_minus).
-           ++ rewrite -> fold_unfold_evaluate_Minus in H_minus.
-              rewrite -> E_ae1 in H_minus.
-              rewrite -> (H_refactor ae).
-              rewrite -> fold_unfold_evaluate_Plus.
-              rewrite -> fold_unfold_evaluate_Minus.
-              rewrite -> E_ae1.
-              exact (H_minus).
-      * split.
-        intros n s H_minus.
-        destruct IHae1 as [IH1_ae1 [IH2_ae1 IH3_ae1]].
-        destruct IHae2 as [IH1_ae2 [IH2_ae2 IH3_ae2]].
-        -- intro ae.
-           rewrite -> (refactoring_preserves_evaluation_aux ae2 ae).
-           reflexivity.
-        -- intro ae.
-           rewrite -> (refactoring_preserves_evaluation_aux ae1 ae).
-           reflexivity.
-        -- intro ae.
-           case (evaluate ae1) as [n1 | s1] eqn:E_ae1.
-           case (evaluate ae2) as [n2 | s2] eqn:E_ae2.
-           case (evaluate ae) as [n_ae | s_ae] eqn:E_ae.
-           ++ rewrite -> (H_refactor ae).
-              rewrite -> fold_unfold_evaluate_Plus.
-              rewrite -> fold_unfold_evaluate_Minus.
-              rewrite -> E_ae.
-              rewrite -> E_ae2.
-              rewrite -> E_ae1.
-              case (n1 <? n2) eqn:E_lt.
-              ** rewrite -> fold_unfold_evaluate_Minus in H_minus.
-                 rewrite -> E_ae2 in H_minus.
-                 rewrite -> E_ae1 in H_minus.
-                 case (n1 <? n2) eqn:E_lt_minus.
-                 --- intro H_absurd.
-                      discriminate H_absurd.
-                 --- discriminate E_lt.
-              ** rewrite -> fold_unfold_evaluate_Minus in H_minus.
-                 rewrite -> E_ae2 in H_minus.
-                 rewrite -> E_ae1 in H_minus.
-                 case (n1 <? n2) eqn:E_lt_minus.
-                 --- discriminate E_lt.
-                 --- intro H_absurd.
-                      discriminate H_absurd.
-           ++ rewrite -> (H_refactor ae).
-              rewrite -> fold_unfold_evaluate_Plus.
-              rewrite -> fold_unfold_evaluate_Minus.
-              rewrite -> E_ae.
-              rewrite -> E_ae2.
-              rewrite -> E_ae1.
-              case (n1 <? n2) eqn:E_lt.
-              ** rewrite -> fold_unfold_evaluate_Minus in H_minus.
-                 rewrite -> E_ae2 in H_minus.
-                 rewrite -> E_ae1 in H_minus.
-                 case (n1 <? n2) eqn:E_lt_minus.
-                 --- discriminate H_minus.
-                 --- discriminate E_lt.
-              ** intro H_true.
-                 exact (H_true).
-           ++ intros _.
-              rewrite -> fold_unfold_evaluate_Minus in H_minus.
-              rewrite -> E_ae2 in H_minus.
-              rewrite -> E_ae1 in H_minus.
-              discriminate H_minus.
-           ++ intros _.
-              rewrite -> fold_unfold_evaluate_Minus in H_minus.
-              rewrite -> E_ae1 in H_minus.
-              discriminate H_minus.
-        -- intros n1 n2 H_minus.
-           destruct IHae1 as [IH1_ae1 [IH2_ae1 IH3_ae1]].
-           destruct IHae2 as [IH1_ae2 [IH2_ae2 IH3_ae2]].
-           ++ intro ae.
-              rewrite -> (refactoring_preserves_evaluation_aux ae2 ae).
-              reflexivity.
-           ++ intro ae.
-              rewrite -> (refactoring_preserves_evaluation_aux ae1 ae).
-              reflexivity.
-           ++ intro ae.
-              case (evaluate ae1) as [n_ae1 | s_ae1] eqn:E_ae1.
-              case (evaluate ae2) as [n_ae2 | s_ae2] eqn:E_ae2.
-              case (evaluate ae) as [n_ae | s_ae] eqn:E_ae.
-              ** intros H_exp_n_ae_eq_exp_n2.
-                 rewrite -> fold_unfold_evaluate_Minus in H_minus.
-                 rewrite -> E_ae2 in H_minus.
-                 rewrite -> E_ae1 in H_minus.
-                 rewrite -> (H_refactor ae).
-                 rewrite -> fold_unfold_evaluate_Plus.
-                 rewrite -> fold_unfold_evaluate_Minus.
-                 rewrite -> E_ae2.
-                 rewrite -> E_ae1.
-                 rewrite -> E_ae.
-                 injection H_exp_n_ae_eq_exp_n2.
-                 intro H_n_ae_eq_n2.
-                 rewrite -> H_n_ae_eq_n2.
-                 rewrite -> H_minus.
-                 reflexivity.
-              ** intro H_absurd.
-                 discriminate H_absurd.
-              ** intro H_ae.
-                 rewrite -> fold_unfold_evaluate_Minus in H_minus.
-                 rewrite -> E_ae2 in H_minus.
-                 rewrite -> E_ae1 in H_minus.
-                 discriminate H_minus.
-              ** intro H_ae.
-                 rewrite -> fold_unfold_evaluate_Minus in H_minus.
-                 rewrite -> E_ae1 in H_minus.
-                 discriminate H_minus.
-Qed.
-
-Proposition equivalence_of_the_two_lemmas_for_refactor_case :
+Proposition equivalence_of_the_two_lemmas_for_refactor :
   forall ae : arithmetic_expression,
     (forall s : string,
         evaluate ae = Expressible_msg s ->
@@ -739,55 +374,8 @@ Proof.
       exact (E_s s (eq_refl (Expressible_msg s)) a).
     + Check (E_s s (eq_refl (Expressible_msg s)) a).
       exact (E_s s (eq_refl (Expressible_msg s)) a).
-  - case ae as [ n | ae1 ae2 | ae1 ae2 ].
-    + intro E. (* Literal case *)
-      split.
-      { intros s E_ae_s a.
-        rewrite -> fold_unfold_refactor_aux_Literal.
-        rewrite -> fold_unfold_evaluate_Plus.
-        rewrite -> E_ae_s.
-        reflexivity.
-      }
-      split.
-      { intros n' s E_ae_n' a E_a_s.
-           rewrite -> fold_unfold_refactor_aux_Literal.
-           rewrite -> fold_unfold_evaluate_Plus.
-           rewrite -> E_ae_n'.
-           rewrite -> E_a_s.
-           reflexivity.
-      }
-      { intros n1 n2 E_ae_n a E_a_n.
-        rewrite -> fold_unfold_refactor_aux_Literal.
-        rewrite -> fold_unfold_evaluate_Plus.
-        rewrite -> E_ae_n.
-        rewrite -> E_a_n.
-        reflexivity.
-      }
-    + intro E. (* Plus case *)
-      split.
-      { intros s E_ae_s a.
-        rewrite -> E.
-        rewrite -> fold_unfold_evaluate_Plus.
-        rewrite -> E_ae_s.
-        reflexivity.
-      }
-      split.
-      { intros n' s E_ae_n' a E_a_s.
-           rewrite -> E.
-           rewrite -> fold_unfold_evaluate_Plus.
-           rewrite -> E_ae_n'.
-           rewrite -> E_a_s.
-           reflexivity.
-      }
-      { intros n1 n2 E_ae_n a E_a_n.
-        rewrite -> E.
-        rewrite -> fold_unfold_evaluate_Plus.
-        rewrite -> E_ae_n.
-        rewrite -> E_a_n.
-        reflexivity.
-      }
-    + intro E. (* Minus case *)
-      split.
+  - intro E. 
+    split.
       { intros s E_ae_s a.
         rewrite -> E.
         rewrite -> fold_unfold_evaluate_Plus.
@@ -811,12 +399,51 @@ Proof.
       }
 Qed.
 
-Proposition refactor_is_idempotent :
+(* ***** *)
+
+Fixpoint eqb_arithmetic_expression (ae1 ae2 : arithmetic_expression) : bool :=
+  match ae1 with
+  | Literal n1 =>
+      match ae2 with
+      | Literal n2 =>
+          Nat.eqb n1 n2
+      | _ =>
+          false
+      end
+  | Plus ae11 ae12 => 
+      match ae2 with
+      | Plus ae21 ae22 =>
+          (eqb_arithmetic_expression ae11 ae21) && (eqb_arithmetic_expression ae12 ae22)
+      | _ =>
+          false
+      end
+  | Minus ae11 ae12 =>
+      match ae2 with
+      | Minus ae21 ae22 =>
+          (eqb_arithmetic_expression ae11 ae21) && (eqb_arithmetic_expression ae12 ae22)
+      | _ =>
+          false
+      end
+  end.
+
+Compute (eqb_arithmetic_expression (Literal 1) (Literal 1)).
+Compute (eqb_arithmetic_expression (Literal 1) (Literal 2)).
+Compute (eqb_arithmetic_expression (Plus (Literal 0) (Literal 1)) (Literal 1)).
+Compute (eqb_arithmetic_expression (Literal 1) (Minus (Literal 1) (Literal 0))).
+Compute (eqb_arithmetic_expression (Minus (Literal 1) (Literal 0)) ((Minus (Literal 1) (Literal 0)))).
+Compute (eqb_arithmetic_expression (Minus (Literal 0) (Literal 1)) ((Minus (Literal 0) (Literal 1)))).
+
+Proposition refactor_is_never_idempotent :
   forall (ae : arithmetic_expression),
-      evaluate (refactor ae) = evaluate (refactor (refactor ae)).
+      refactor ae <> refactor (refactor ae).
 Proof.
   intro ae.
-  rewrite -> (refactoring_preserves_evaluation (refactor ae)).
+  unfold refactor.
+  case ae as [ n | ae1 ae2 | ae1 ae2 ].
+  - rewrite -> fold_unfold_refactor_aux_Literal.
+    rewrite -> fold_unfold_refactor_aux_Plus.
+    rewrite ->2 fold_unfold_refactor_aux_Literal.
+    Check (eqb_arithmetic_expression (Plus (Literal n) (Literal 0)) (Plus (Literal n) (Plus (Literal 0)(Literal 0)))).
   reflexivity.
 Qed.
 
